<?xml version="1.0"?>


<!-- Copyright (c) 2014 Engineering Ingegneria Informatica s.p.a. 
   - This Source Code Form is subject to the terms of the Mozilla Public
   - License, v. 2.0. If a copy of the MPL was not distributed with this
   - file, You can obtain one at http://mozilla.org/MPL/2.0/. -->
   

<!DOCTYPE rdf:RDF [
    <!ENTITY owl "http://www.w3.org/2002/07/owl#" >
    <!ENTITY xsd "http://www.w3.org/2001/XMLSchema#" >
    <!ENTITY rdfs "http://www.w3.org/2000/01/rdf-schema#" >
    <!ENTITY rdf "http://www.w3.org/1999/02/22-rdf-syntax-ns#" >
    <!ENTITY mweb "http://www.markosproject.eu/ontologies/web#" >
    <!ENTITY mtop "http://www.markosproject.eu/ontologies/top#" >
    <!ENTITY msw "http://www.markosproject.eu/ontologies/software#" >
]>


<rdf:RDF xmlns="http://www.markosproject.eu/ontologies/web#"
     xml:base="http://www.markosproject.eu/ontologies/web"
     xmlns:rdfs="http://www.w3.org/2000/01/rdf-schema#"
     xmlns:mweb="http://www.markosproject.eu/ontologies/web#"
     xmlns:owl="http://www.w3.org/2002/07/owl#"
     xmlns:xsd="http://www.w3.org/2001/XMLSchema#"
     xmlns:rdf="http://www.w3.org/1999/02/22-rdf-syntax-ns#"
     xmlns:msw="http://www.markosproject.eu/ontologies/software#"
     xmlns:mtop="http://www.markosproject.eu/ontologies/top#">
    <owl:Ontology rdf:about="http://www.markosproject.eu/ontologies/web">
        <owl:imports rdf:resource="&msw;2014/09/30"/>
        <owl:versionIRI rdf:resource="&mweb;2014/09/30"/>
    </owl:Ontology>
    


    <!-- 
    ///////////////////////////////////////////////////////////////////////////////////////
    //
    // Object Properties
    //
    ///////////////////////////////////////////////////////////////////////////////////////
     -->

    


    <!-- http://www.markosproject.eu/ontologies/web#embeddedScript -->

    <owl:ObjectProperty rdf:about="&mweb;embeddedScript">
        <rdfs:label xml:lang="en">Embedded script</rdfs:label>
        <rdfs:comment xml:lang="en">Script program embedded within the subjct HTMLPage.</rdfs:comment>
        <rdfs:subPropertyOf rdf:resource="&msw;usedSoftwareEntity"/>
        <rdfs:subPropertyOf rdf:resource="&mtop;containedEntity"/>
        <rdfs:domain rdf:resource="&mweb;WebPageComponent"/>
        <rdfs:range rdf:resource="&mweb;WebScript"/>
    </owl:ObjectProperty>
    


    <!-- http://www.markosproject.eu/ontologies/web#externalUsedScript -->

    <owl:ObjectProperty rdf:about="&mweb;externalUsedScript">
        <rdfs:label xml:lang="en">External used Script</rdfs:label>
        <rdfs:comment xml:lang="en">Any WebScript program that is used by the subject WebPageComponent but is not embedded in it.

If an HTMLFile has a referredScriptFile then the referredScriptFile is the manifestation of a usedScript of the HTMLPAge manifested by the HTMLFile (and viceversa). </rdfs:comment>
        <rdfs:subPropertyOf rdf:resource="&msw;usedSoftwareEntity"/>
        <rdfs:domain rdf:resource="&mweb;WebPageComponent"/>
        <rdfs:range rdf:resource="&mweb;WebScript"/>
    </owl:ObjectProperty>
    


    <!-- http://www.markosproject.eu/ontologies/web#referredScriptFile -->

    <owl:ObjectProperty rdf:about="&mweb;referredScriptFile">
        <rdfs:label xml:lang="en">Referred Script file</rdfs:label>
        <rdfs:comment xml:lang="en">Any Script file that is referred by the subject HTML page (e.g. through the &quot;src&quot; attribute of a SCRIPT element).</rdfs:comment>
        <rdfs:range rdf:resource="&msw;ScriptFile"/>
        <rdfs:subPropertyOf rdf:resource="&mtop;usedEntity"/>
        <rdfs:domain rdf:resource="&mweb;WebPageSourceCodeFile"/>
        <owl:propertyChainAxiom rdf:parseType="Collection">
            <rdf:Description>
                <owl:inverseOf rdf:resource="&msw;manifestation"/>
            </rdf:Description>
            <rdf:Description rdf:about="&mweb;externalUsedScript"/>
            <rdf:Description rdf:about="&msw;manifestation"/>
        </owl:propertyChainAxiom>
    </owl:ObjectProperty>
    


    <!-- 
    ///////////////////////////////////////////////////////////////////////////////////////
    //
    // Data properties
    //
    ///////////////////////////////////////////////////////////////////////////////////////
     -->

    


    <!-- http://www.markosproject.eu/ontologies/web#url -->

    <owl:DatatypeProperty rdf:about="&mweb;url">
        <rdf:type rdf:resource="&owl;FunctionalProperty"/>
        <rdfs:label xml:lang="en">Location</rdfs:label>
        <rdfs:seeAlso rdf:datatype="&xsd;anyURI">http://www.w3.org/DesignIssues/HTTP-URI2.html</rdfs:seeAlso>
        <rdfs:comment xml:lang="en">The URL (also URI) of the subject Web Document (a client performing an HTTP request at this URL must receive an HTTP response code of 200).
</rdfs:comment>
        <rdfs:domain rdf:resource="&mweb;WebDocument"/>
        <rdfs:range rdf:resource="&xsd;anyURI"/>
    </owl:DatatypeProperty>
    


    <!-- 
    ///////////////////////////////////////////////////////////////////////////////////////
    //
    // Classes
    //
    ///////////////////////////////////////////////////////////////////////////////////////
     -->

    


    <!-- http://www.markosproject.eu/ontologies/web#ApplicationServer -->

    <owl:Class rdf:about="&mweb;ApplicationServer">
        <rdfs:subClassOf rdf:resource="&mweb;WebServer"/>
        <rdfs:comment xml:lang="en">Any extensible ServerProgram dedicated to the implementation of specific kind of distributed applications (i.e. programs), including web applications.</rdfs:comment>
    </owl:Class>
    


    <!-- http://www.markosproject.eu/ontologies/web#ClientProgram -->

    <owl:Class rdf:about="&mweb;ClientProgram">
        <rdfs:label xml:lang="en">Client program</rdfs:label>
        <rdfs:subClassOf rdf:resource="&msw;Program"/>
        <rdfs:comment xml:lang="en">Any Program to uses specific services provided by some (Server) Program. A ClientProgram may be extensible by means of specific kind of data/content and components.</rdfs:comment>
    </owl:Class>
    


    <!-- http://www.markosproject.eu/ontologies/web#ClientSideWebComponent -->

    <owl:Class rdf:about="&mweb;ClientSideWebComponent">
        <rdfs:label xml:lang="en">Web client component</rdfs:label>
        <rdfs:subClassOf rdf:resource="&mweb;WebComponent"/>
        <rdfs:comment xml:lang="en">Any Component that runs in a web browser (e.g. Java Applets, a SilverLight control).</rdfs:comment>
    </owl:Class>
    


    <!-- http://www.markosproject.eu/ontologies/web#HTMLFile -->

    <owl:Class rdf:about="&mweb;HTMLFile">
        <rdfs:label xml:lang="en">HTML file</rdfs:label>
        <owl:equivalentClass>
            <owl:Class>
                <owl:intersectionOf rdf:parseType="Collection">
                    <rdf:Description rdf:about="&msw;SourceCodeFile"/>
                    <owl:Restriction>
                        <owl:onProperty rdf:resource="&msw;codingLanguage"/>
                        <owl:hasValue rdf:resource="&msw;HTML_LANGUAGE"/>
                    </owl:Restriction>
                </owl:intersectionOf>
            </owl:Class>
        </owl:equivalentClass>
        <rdfs:subClassOf rdf:resource="&mweb;WebPageSourceCodeFile"/>
        <rdfs:comment xml:lang="en">Any SourceCodeFile written in the HTML language.</rdfs:comment>
    </owl:Class>
    


    <!-- http://www.markosproject.eu/ontologies/web#HTMLPage -->

    <owl:Class rdf:about="&mweb;HTMLPage">
        <rdfs:label xml:lang="en">HTML page</rdfs:label>
        <owl:equivalentClass>
            <owl:Class>
                <owl:intersectionOf rdf:parseType="Collection">
                    <rdf:Description rdf:about="&msw;SoftwareEntity"/>
                    <owl:Restriction>
                        <owl:onProperty rdf:resource="&msw;sourceCode"/>
                        <owl:allValuesFrom rdf:resource="&mweb;HTMLFile"/>
                    </owl:Restriction>
                </owl:intersectionOf>
            </owl:Class>
        </owl:equivalentClass>
        <rdfs:subClassOf rdf:resource="&mweb;WebPageComponent"/>
        <rdfs:comment xml:lang="en">Any abstract document implemented using the HTML programming language.</rdfs:comment>
    </owl:Class>
    


    <!-- http://www.markosproject.eu/ontologies/web#ServerProgram -->

    <owl:Class rdf:about="&mweb;ServerProgram">
        <rdfs:subClassOf rdf:resource="&msw;Program"/>
        <rdfs:comment xml:lang="en">Any Program to provide specific kind of services to requesters running programs (Clients). A ServerProgram may be extensible by means of specific kind of data/content and components. </rdfs:comment>
    </owl:Class>
    


    <!-- http://www.markosproject.eu/ontologies/web#ServerSideComponent -->

    <owl:Class rdf:about="&mweb;ServerSideComponent">
        <rdfs:subClassOf rdf:resource="&msw;Component"/>
        <rdfs:comment xml:lang="en">Any Component that runs under the control of an ApplicationServer and extends its capabilities (e.g. a SCA component).</rdfs:comment>
    </owl:Class>
    


    <!-- http://www.markosproject.eu/ontologies/web#ServerSideWebComponent -->

    <owl:Class rdf:about="&mweb;ServerSideWebComponent">
        <rdfs:label xml:lang="en">Web server component</rdfs:label>
        <rdfs:subClassOf rdf:resource="&mweb;ServerSideComponent"/>
        <rdfs:subClassOf rdf:resource="&mweb;WebComponent"/>
        <rdfs:comment xml:lang="en">Any Component that runs under the control of a WebServer and extends its capabilities (e.g., ASP pages, Java HTTP Servlets, PHP pages). A ServerSideWebComponent may include some ClientSideWebComponent to be sent to web clients.</rdfs:comment>
    </owl:Class>
    


    <!-- http://www.markosproject.eu/ontologies/web#WebApplication -->

    <owl:Class rdf:about="&mweb;WebApplication">
        <rdfs:label xml:lang="en">Web application</rdfs:label>
        <owl:equivalentClass>
            <owl:Class>
                <owl:intersectionOf rdf:parseType="Collection">
                    <rdf:Description rdf:about="&msw;Program"/>
                    <owl:Restriction>
                        <owl:onProperty rdf:resource="&mtop;containedEntity"/>
                        <owl:someValuesFrom rdf:resource="&mweb;WebComponent"/>
                    </owl:Restriction>
                </owl:intersectionOf>
            </owl:Class>
        </owl:equivalentClass>
        <rdfs:comment xml:lang="en">Any Program containing one or more WebComponents (altogheter implementing a coherent set of functionalities accessed by final users by means of a web browser).</rdfs:comment>
    </owl:Class>
    


    <!-- http://www.markosproject.eu/ontologies/web#WebBrowser -->

    <owl:Class rdf:about="&mweb;WebBrowser">
        <rdfs:label xml:lang="en">Web browser</rdfs:label>
        <rdfs:subClassOf rdf:resource="&mweb;WebClient"/>
        <rdfs:seeAlso rdf:datatype="&xsd;anyURI">http://en.wikipedia.org/w/index.php?title=Web_browser&amp;oldid=602376902</rdfs:seeAlso>
        <rdfs:comment xml:lang="en">A software application (also called web client) for retrieving, presenting and traversing information resources (i.e web documents) on the World Wide Web.</rdfs:comment>
    </owl:Class>
    


    <!-- http://www.markosproject.eu/ontologies/web#WebClient -->

    <owl:Class rdf:about="&mweb;WebClient">
        <rdfs:label xml:lang="en">Web client</rdfs:label>
        <rdfs:subClassOf rdf:resource="&mweb;ClientProgram"/>
        <rdfs:comment xml:lang="en">Any Program that runs on the user side of the Web. It may be a Web browser or another application accessing the services provided by WebServers.</rdfs:comment>
    </owl:Class>
    


    <!-- http://www.markosproject.eu/ontologies/web#WebComponent -->

    <owl:Class rdf:about="&mweb;WebComponent">
        <rdfs:label xml:lang="en">Web component</rdfs:label>
        <owl:equivalentClass>
            <owl:Class>
                <owl:unionOf rdf:parseType="Collection">
                    <rdf:Description rdf:about="&mweb;ClientSideWebComponent"/>
                    <rdf:Description rdf:about="&mweb;ServerSideWebComponent"/>
                </owl:unionOf>
            </owl:Class>
        </owl:equivalentClass>
        <rdfs:subClassOf rdf:resource="&msw;Component"/>
        <owl:disjointWith rdf:resource="&mweb;WebDocument"/>
        <rdfs:comment xml:lang="en">A WebClient Component or a WebServerComponent.</rdfs:comment>
    </owl:Class>
    


    <!-- http://www.markosproject.eu/ontologies/web#WebDocument -->

    <owl:Class rdf:about="&mweb;WebDocument">
        <rdfs:label xml:lang="en">Web document</rdfs:label>
        <rdfs:subClassOf rdf:resource="&msw;SoftwareArtifact"/>
        <rdfs:seeAlso rdf:datatype="&xsd;anyURI">http://www.w3.org/TR/cooluris/#oldweb</rdfs:seeAlso>
        <rdfs:comment xml:lang="en">Anything available on the web, identified by its own URI, and that can be conveyed in a message.
&quot;Every Web document has its own URI. Note that a Web document is not the same as a file: a single Web document can be available in many different formats and languages, and a single file, for example a PHP script, may be responsible for generating a large number of Web documents with different URIs. A Web document is defined as something that has a URI and can return representations (responses in a format such as HTML or JPEG or RDF) of the identified resource in response to HTTP requests.In technical literature [...] the term Information Resource is used instead of Web document&quot; 


A WebDocument is not a WebComponent, but a WebComponent may produce/implement a WebPage.</rdfs:comment>
    </owl:Class>
    


    <!-- http://www.markosproject.eu/ontologies/web#WebPage -->

    <owl:Class rdf:about="&mweb;WebPage">
        <rdfs:label xml:lang="en">Web page</rdfs:label>
        <rdfs:subClassOf rdf:resource="&mweb;WebDocument"/>
        <rdfs:subClassOf>
            <owl:Restriction>
                <owl:onProperty>
                    <rdf:Description>
                        <owl:inverseOf rdf:resource="&msw;manifestation"/>
                    </rdf:Description>
                </owl:onProperty>
                <owl:allValuesFrom rdf:resource="&mweb;HTMLPage"/>
            </owl:Restriction>
        </rdfs:subClassOf>
        <rdfs:seeAlso rdf:datatype="&xsd;anyURI">http://en.wikipedia.org/w/index.php?title=Web_page&amp;oldid=544129970</rdfs:seeAlso>
        <rdfs:comment xml:lang="en">Any web document implemented by an HTMLPage and related tecnlogies. A WebPage have a specific URI. Same content published at two different URI corresponds to two different WebPages. 

Note that an WebPage and an HTMLFile are different kind of manifestations of HTMLPage. Different WebPages (having different URI) may show the same HTMLPage (i.e. may have same content) and different HTMLFiles (having a different fyle system path) may contain the source code of the same HTMLPage .</rdfs:comment>
    </owl:Class>
    


    <!-- http://www.markosproject.eu/ontologies/web#WebPageComponent -->

    <owl:Class rdf:about="&mweb;WebPageComponent">
        <rdfs:subClassOf rdf:resource="&mweb;ClientSideWebComponent"/>
        <rdfs:comment xml:lang="en">Any WebComponent that implements a WebPage (i.e. any HTMLPage or any component that produces HTML code).  

A .net ASP or a Java JSP are examples of WebPageComponents.</rdfs:comment>
    </owl:Class>
    


    <!-- http://www.markosproject.eu/ontologies/web#WebPageSourceCodeFile -->

    <owl:Class rdf:about="&mweb;WebPageSourceCodeFile">
        <rdfs:label xml:lang="en">Web Page source code file</rdfs:label>
        <rdfs:subClassOf rdf:resource="&msw;SourceCodeFile"/>
        <rdfs:comment xml:lang="en">Any source code file of a WebPageComponent </rdfs:comment>
    </owl:Class>
    


    <!-- http://www.markosproject.eu/ontologies/web#WebScript -->

    <owl:Class rdf:about="&mweb;WebScript">
        <rdfs:label xml:lang="en">WebScript</rdfs:label>
        <rdfs:subClassOf rdf:resource="&msw;Program"/>
        <rdfs:subClassOf rdf:resource="&mweb;ClientSideWebComponent"/>
        <rdfs:comment xml:lang="en">Any Program that may be emebedded or delivered with an HTML Page and which source code may be interpreted by a web browser.</rdfs:comment>
    </owl:Class>
    


    <!-- http://www.markosproject.eu/ontologies/web#WebServer -->

    <owl:Class rdf:about="&mweb;WebServer">
        <rdfs:label xml:lang="en">Web server</rdfs:label>
        <rdfs:subClassOf rdf:resource="&mweb;ServerProgram"/>
        <rdfs:comment xml:lang="en">Any ServerProgram that stores, processes and delivers web pages to any client performing requests using the Hypertext Transfer Protocol (HTTP).</rdfs:comment>
    </owl:Class>
</rdf:RDF>



<!-- Generated by the OWL API (version 3.4.2) http://owlapi.sourceforge.net -->

