<?xml version="1.0"?>

<!-- Copyright (c) 2014 Fraunhofer Gesellschaft 
   - This Source Code Form is subject to the terms of the Mozilla Public
   - License, v. 2.0. If a copy of the MPL was not distributed with this
   - file, You can obtain one at http://mozilla.org/MPL/2.0/. -->
   
<!DOCTYPE rdf:RDF [
    <!ENTITY terms "http://purl.org/dc/terms/" >
    <!ENTITY owl "http://www.w3.org/2002/07/owl#" >
    <!ENTITY xsd "http://www.w3.org/2001/XMLSchema#" >
    <!ENTITY rdfs "http://www.w3.org/2000/01/rdf-schema#" >
    <!ENTITY rdf "http://www.w3.org/1999/02/22-rdf-syntax-ns#" >
    <!ENTITY mlic "http://www.markosproject.eu/ontologies/licenses#" >
]>


<rdf:RDF xmlns="http://www.markosproject.eu/ontologies/licenses#"
     xml:base="http://www.markosproject.eu/ontologies/licenses"
     xmlns:rdfs="http://www.w3.org/2000/01/rdf-schema#"
     xmlns:terms="http://purl.org/dc/terms/"
     xmlns:owl="http://www.w3.org/2002/07/owl#"
     xmlns:xsd="http://www.w3.org/2001/XMLSchema#"
     xmlns:rdf="http://www.w3.org/1999/02/22-rdf-syntax-ns#"
     xmlns:mlic="http://www.markosproject.eu/ontologies/licenses#">
    <owl:Ontology rdf:about="http://www.markosproject.eu/ontologies/licenses">
        <owl:versionIRI rdf:resource="&mlic;2014/10/07"/>
        <owl:imports rdf:resource="http://www.markosproject.eu/ontologies/top#2014/10/07"/>
    </owl:Ontology>
    


    <!-- 
    ///////////////////////////////////////////////////////////////////////////////////////
    //
    // Annotation properties
    //
    ///////////////////////////////////////////////////////////////////////////////////////
     -->

    


    <!-- http://purl.org/dc/terms/created -->

    <owl:AnnotationProperty rdf:about="&terms;created"/>
    


    <!-- http://purl.org/dc/terms/creator -->

    <owl:AnnotationProperty rdf:about="&terms;creator">
        <rdfs:subPropertyOf rdf:resource="&terms;creator"/>
    </owl:AnnotationProperty>
    


    <!-- http://purl.org/dc/terms/publisher -->

    <owl:AnnotationProperty rdf:about="&terms;publisher"/>
    


    <!-- http://www.markosproject.eu/ontologies/licenses#creationDate -->

    <owl:AnnotationProperty rdf:about="&mlic;creationDate">
        <rdfs:label xml:lang="en">Creation date</rdfs:label>
        <rdfs:comment xml:lang="en">Date when the subject license assessment was created.</rdfs:comment>
        <rdfs:subPropertyOf rdf:resource="&terms;created"/>
        <rdfs:domain rdf:resource="&mlic;LicenseAssessment"/>
        <rdfs:range rdf:resource="&xsd;dateTime"/>
    </owl:AnnotationProperty>
    


    <!-- http://www.markosproject.eu/ontologies/licenses#creator -->

    <owl:AnnotationProperty rdf:about="&mlic;creator">
        <rdfs:label xml:lang="en">Creator</rdfs:label>
        <rdfs:comment xml:lang="en">Username of the user (it may be also an automatic agent) that created the subject LicenseAssessment on the analysesTool. In particular, if the value is an empty string, than the LicenseAssessment has been done from a default automatic agent provided by the analysesTool.</rdfs:comment>
        <rdfs:subPropertyOf rdf:resource="&terms;creator"/>
        <rdfs:domain rdf:resource="&mlic;LicenseAssessment"/>
        <rdfs:range rdf:resource="&xsd;string"/>
    </owl:AnnotationProperty>
    


    <!-- http://www.markosproject.eu/ontologies/licenses#publisher -->

    <owl:AnnotationProperty rdf:about="&mlic;publisher">
        <rdfs:label xml:lang="en">Analyses tool</rdfs:label>
        <rdfs:comment xml:lang="en">Organization or single agent that publishes the subject LicenseAssessment.</rdfs:comment>
        <rdfs:range rdf:resource="&terms;Agent"/>
        <rdfs:subPropertyOf rdf:resource="&terms;publisher"/>
        <rdfs:domain rdf:resource="&mlic;LicenseAssessment"/>
    </owl:AnnotationProperty>
    


    <!-- 
    ///////////////////////////////////////////////////////////////////////////////////////
    //
    // Object Properties
    //
    ///////////////////////////////////////////////////////////////////////////////////////
     -->

    


    <!-- http://www.markosproject.eu/ontologies/licenses#assessedLicense -->

    <owl:ObjectProperty rdf:about="&mlic;assessedLicense">
        <rdf:type rdf:resource="&owl;FunctionalProperty"/>
        <rdfs:label xml:lang="en">Assessed license</rdfs:label>
        <rdfs:comment xml:lang="en">The CopyrightLicense that has been assessed (note that a same Entity may be covered by more than one CopyrightLicense).</rdfs:comment>
        <rdfs:range rdf:resource="&mlic;CopyrightLicense"/>
        <rdfs:domain rdf:resource="&mlic;LicenseAssessment"/>
    </owl:ObjectProperty>
    


    <!-- http://www.markosproject.eu/ontologies/licenses#assessedLicenseTemplate -->

    <owl:ObjectProperty rdf:about="&mlic;assessedLicenseTemplate">
        <rdf:type rdf:resource="&owl;FunctionalProperty"/>
        <rdfs:label xml:lang="en">Assessed license template</rdfs:label>
        <rdfs:comment xml:lang="en">The CopyrightLicenseTemplate that has been assessed (note that a same Entity may be covered by several CopyrightLicenses adopting different LicenseTemplates).</rdfs:comment>
        <rdfs:range rdf:resource="&mlic;CopyrightLicenseTemplate"/>
        <rdfs:domain rdf:resource="&mlic;LicenseAssessment"/>
    </owl:ObjectProperty>
    


    <!-- http://www.markosproject.eu/ontologies/licenses#coveringLicense -->

    <owl:ObjectProperty rdf:about="&mlic;coveringLicense">
        <rdfs:label xml:lang="en">Covering license</rdfs:label>
        <rdfs:comment xml:lang="en">The CopyrightLicense that regulates the usage of the subject Entity, i.e. the CopyrightLicense of the Work that the Entity is a legal part of.

This ontology distinguish the legal parts of an Entity from other parts of the Entity, i.e. an Entity may contain parts that are not legal parts. 

The CopyrightLicense of an entity applies to all (and only) its legal parts.

A Work may have only legal parts. All legal parts of an Entity are parts of a same Work and that Entity is a legal part of that Work.

 </rdfs:comment>
        <rdfs:range rdf:resource="&mlic;CopyrightLicense"/>
        <rdfs:domain rdf:resource="http://www.markosproject.eu/ontologies/top#Entity"/>
    </owl:ObjectProperty>
    


    <!-- http://www.markosproject.eu/ontologies/licenses#coveringLicenseAssessment -->

    <owl:ObjectProperty rdf:about="&mlic;coveringLicenseAssessment">
        <rdf:type rdf:resource="&owl;InverseFunctionalProperty"/>
        <rdfs:label xml:lang="en">License assessment</rdfs:label>
        <rdfs:comment xml:lang="en">Assessment of the compliance of the license of the subject Entity with respect to the licenses of the used (elements of) works.</rdfs:comment>
        <rdfs:range rdf:resource="&mlic;LicenseAssessment"/>
        <rdfs:domain rdf:resource="http://www.markosproject.eu/ontologies/top#Entity"/>
    </owl:ObjectProperty>
    


    <!-- http://www.markosproject.eu/ontologies/licenses#licenseTemplate -->

    <owl:ObjectProperty rdf:about="&mlic;licenseTemplate">
        <rdfs:label xml:lang="en">License template </rdfs:label>
        <rdfs:comment xml:lang="en">The the template of the coveringLicense of the subject Work (the property &quot;licenseTemplate&quot; is equivalent to the chain &quot;coveringLicense o template&quot;).</rdfs:comment>
        <rdfs:range rdf:resource="&mlic;CopyrightLicenseTemplate"/>
        <rdfs:domain rdf:resource="http://www.markosproject.eu/ontologies/top#Entity"/>
        <owl:propertyChainAxiom rdf:parseType="Collection">
            <rdf:Description rdf:about="&mlic;coveringLicense"/>
            <rdf:Description rdf:about="&mlic;template"/>
        </owl:propertyChainAxiom>
    </owl:ObjectProperty>
    


    <!-- http://www.markosproject.eu/ontologies/licenses#template -->

    <owl:ObjectProperty rdf:about="&mlic;template">
        <rdf:type rdf:resource="&owl;FunctionalProperty"/>
        <rdfs:label xml:lang="en">Template</rdfs:label>
        <rdfs:comment xml:lang="en">The CopyrightLicenseTemplate the sucject CopyrightLicense conforms to. </rdfs:comment>
        <rdfs:domain rdf:resource="&mlic;CopyrightLicense"/>
        <rdfs:range rdf:resource="&mlic;CopyrightLicenseTemplate"/>
    </owl:ObjectProperty>
    


    <!-- 
    ///////////////////////////////////////////////////////////////////////////////////////
    //
    // Data properties
    //
    ///////////////////////////////////////////////////////////////////////////////////////
     -->

    


    <!-- http://www.markosproject.eu/ontologies/licenses#analyses -->

    <owl:DatatypeProperty rdf:about="&mlic;analyses">
        <rdf:type rdf:resource="&owl;FunctionalProperty"/>
        <rdfs:label xml:lang="en">Analyses</rdfs:label>
        <rdfs:comment xml:lang="en">Description of the reasoning supporting the assessment result (see Data Property :isLicenseCompliant).</rdfs:comment>
        <rdfs:domain rdf:resource="&mlic;LicenseAssessment"/>
        <rdfs:range rdf:resource="&xsd;string"/>
    </owl:DatatypeProperty>
    


    <!-- http://www.markosproject.eu/ontologies/licenses#argumentGraph -->

    <owl:DatatypeProperty rdf:about="&mlic;argumentGraph">
        <rdf:type rdf:resource="&owl;FunctionalProperty"/>
        <rdfs:label xml:lang="en">Argument graph</rdfs:label>
        <rdfs:comment xml:lang="en">Web address where an argument graph supporting the assessment is published.</rdfs:comment>
        <rdfs:domain rdf:resource="&mlic;LicenseAssessment"/>
        <rdfs:range rdf:resource="&xsd;anyURI"/>
    </owl:DatatypeProperty>
    


    <!-- http://www.markosproject.eu/ontologies/licenses#isLicenseCompliant -->

    <owl:DatatypeProperty rdf:about="&mlic;isLicenseCompliant">
        <rdf:type rdf:resource="&owl;FunctionalProperty"/>
        <rdfs:label xml:lang="en">Is license compliant</rdfs:label>
        <rdfs:comment xml:lang="en">The result of the license assessment: it is true if the assessed license is compliant with the other involved licenses, otherwise it is false.</rdfs:comment>
        <rdfs:domain rdf:resource="&mlic;LicenseAssessment"/>
        <rdfs:range rdf:resource="&xsd;boolean"/>
    </owl:DatatypeProperty>
    


    <!-- 
    ///////////////////////////////////////////////////////////////////////////////////////
    //
    // Classes
    //
    ///////////////////////////////////////////////////////////////////////////////////////
     -->

    


    <!-- http://www.markosproject.eu/ontologies/licenses#CopyrightLicense -->

    <owl:Class rdf:about="&mlic;CopyrightLicense">
        <rdfs:label xml:lang="en">Copyright license</rdfs:label>
        <rdfs:subClassOf rdf:resource="http://www.markosproject.eu/ontologies/top#Entity"/>
        <rdfs:comment xml:lang="en">Any individual license, with which a particular legal entity, the licensor, grants rights to another legal entity, the licensee.</rdfs:comment>
    </owl:Class>
    


    <!-- http://www.markosproject.eu/ontologies/licenses#CopyrightLicenseTemplate -->

    <owl:Class rdf:about="&mlic;CopyrightLicenseTemplate">
        <rdfs:label xml:lang="en">Copyright license template</rdfs:label>
        <rdfs:subClassOf rdf:resource="http://www.markosproject.eu/ontologies/top#NamedEntity"/>
        <rdfs:comment xml:lang="en">Any software license templates, such as GPL or BSD. A particular copyright  license can be an instance of such a template.</rdfs:comment>
    </owl:Class>
    


    <!-- http://www.markosproject.eu/ontologies/licenses#LicenseAssessment -->

    <owl:Class rdf:about="&mlic;LicenseAssessment">
        <rdfs:label xml:lang="en">License assessment</rdfs:label>
        <rdfs:subClassOf rdf:resource="http://www.markosproject.eu/ontologies/top#Entity"/>
        <rdfs:comment xml:lang="en">Assessment of the compliance of a license of an Entity with respect to the licenses of the used Entities.</rdfs:comment>
    </owl:Class>
    


    <!-- http://www.markosproject.eu/ontologies/licenses#Work -->

    <owl:Class rdf:about="&mlic;Work">
        <rdfs:label xml:lang="en">Work</rdfs:label>
        <rdfs:subClassOf rdf:resource="http://www.markosproject.eu/ontologies/top#Entity"/>
        <rdfs:comment xml:lang="en">Any literary and/or artistic work that may be offered under the terms of a License, including without limitation any production in the literary, scientific and artistic domain, whatever may be the mode or form of its expression including digital form, such as a book, pamphlet and other writing; a lecture, address, sermon or other work of the same nature; a dramatic or dramatico-musical work; a choreographic work or entertainment in dumb show; a musical composition with or without words; a cinematographic work to which are assimilated works expressed by a process analogous to cinematography; a work of drawing, painting, architecture, sculpture, engraving or lithography; a photographic work to which are assimilated works expressed by a process analogous to photography; a work of applied art; an illustration, map, plan, sketch or three-dimensional work relative to geography, topography, architecture or science; a performance; a broadcast; a phonogram; a compilation of data to the extent it is protected as a copyrightable work; or a work performed by a variety or circus performer to the extent it is not otherwise considered a literary or artistic work.</rdfs:comment>
    </owl:Class>
</rdf:RDF>



<!-- Generated by the OWL API (version 3.4.2) http://owlapi.sourceforge.net -->

