<?xml version="1.0"?>


<!DOCTYPE rdf:RDF [
    <!ENTITY owl "http://www.w3.org/2002/07/owl#" >
    <!ENTITY xsd "http://www.w3.org/2001/XMLSchema#" >
    <!ENTITY rdfs "http://www.w3.org/2000/01/rdf-schema#" >
    <!ENTITY rdf "http://www.w3.org/1999/02/22-rdf-syntax-ns#" >
]>


<rdf:RDF xmlns="http://www.markosproject.eu/ontologies/licenses#"
     xml:base="http://www.markosproject.eu/ontologies/licenses"
     xmlns:rdfs="http://www.w3.org/2000/01/rdf-schema#"
     xmlns:owl="http://www.w3.org/2002/07/owl#"
     xmlns:xsd="http://www.w3.org/2001/XMLSchema#"
     xmlns:rdf="http://www.w3.org/1999/02/22-rdf-syntax-ns#">
    <owl:Ontology rdf:about="http://www.markosproject.eu/ontologies/licenses"/>
    


    <!-- 
    ///////////////////////////////////////////////////////////////////////////////////////
    //
    // Object Properties
    //
    ///////////////////////////////////////////////////////////////////////////////////////
     -->

    


    <!-- http://www.markosproject.eu/ontologies/licenses#assessment -->

    <owl:ObjectProperty rdf:about="http://www.markosproject.eu/ontologies/licenses#assessment">
        <rdfs:label xml:lang="en">Assessment</rdfs:label>
        <rdfs:comment xml:lang="en">Assessment of the compliance of the subject license with respect to the licenses of the works used by the work associated to the subject license.</rdfs:comment>
        <rdfs:domain rdf:resource="http://www.markosproject.eu/ontologies/licenses#CopyrightLicense"/>
        <rdfs:range rdf:resource="http://www.markosproject.eu/ontologies/licenses#LicenseAssessment"/>
    </owl:ObjectProperty>
    


    <!-- http://www.markosproject.eu/ontologies/licenses#coveringLicense -->

    <owl:ObjectProperty rdf:about="http://www.markosproject.eu/ontologies/licenses#coveringLicense">
        <rdfs:label xml:lang="en">Covering license</rdfs:label>
        <rdfs:comment xml:lang="en">The CopyrightLicense that regulate the usage of the subject Work.</rdfs:comment>
        <rdfs:range rdf:resource="http://www.markosproject.eu/ontologies/licenses#CopyrightLicense"/>
        <rdfs:domain rdf:resource="http://www.markosproject.eu/ontologies/licenses#Work"/>
    </owl:ObjectProperty>
    


    <!-- http://www.markosproject.eu/ontologies/licenses#template -->

    <owl:ObjectProperty rdf:about="http://www.markosproject.eu/ontologies/licenses#template">
        <rdfs:label xml:lang="en">Template</rdfs:label>
        <rdfs:comment xml:lang="en">The CopyrightLicenseTemplate the sucject CopyrightLicense conforms to. </rdfs:comment>
        <rdfs:domain rdf:resource="http://www.markosproject.eu/ontologies/licenses#CopyrightLicense"/>
    </owl:ObjectProperty>
    


    <!-- 
    ///////////////////////////////////////////////////////////////////////////////////////
    //
    // Data properties
    //
    ///////////////////////////////////////////////////////////////////////////////////////
     -->

    


    <!-- http://www.markosproject.eu/ontologies/licenses#argumentation -->

    <owl:DatatypeProperty rdf:about="http://www.markosproject.eu/ontologies/licenses#argumentation">
        <rdf:type rdf:resource="&owl;FunctionalProperty"/>
        <rdfs:comment xml:lang="en">Argumentation</rdfs:comment>
        <rdfs:comment xml:lang="en">Description of the reasoning supporting the assessment result (see Data Property :isLicenseCompliant).</rdfs:comment>
        <rdfs:domain rdf:resource="http://www.markosproject.eu/ontologies/licenses#LicenseAssessment"/>
        <rdfs:range rdf:resource="&xsd;string"/>
    </owl:DatatypeProperty>
    


    <!-- http://www.markosproject.eu/ontologies/licenses#isLicenseCompliant -->

    <owl:DatatypeProperty rdf:about="http://www.markosproject.eu/ontologies/licenses#isLicenseCompliant">
        <rdf:type rdf:resource="&owl;FunctionalProperty"/>
        <rdfs:label xml:lang="en">Is license compliant</rdfs:label>
        <rdfs:comment xml:lang="en">The result of the license assessment: it is true if the assessed license is compliant with the other involved licenses, otherwise it is false.</rdfs:comment>
        <rdfs:domain rdf:resource="http://www.markosproject.eu/ontologies/licenses#LicenseAssessment"/>
        <rdfs:range rdf:resource="&xsd;boolean"/>
    </owl:DatatypeProperty>
    


    <!-- 
    ///////////////////////////////////////////////////////////////////////////////////////
    //
    // Classes
    //
    ///////////////////////////////////////////////////////////////////////////////////////
     -->

    


    <!-- http://www.markosproject.eu/ontologies/licenses#CopyrightLicense -->

    <owl:Class rdf:about="http://www.markosproject.eu/ontologies/licenses#CopyrightLicense">
        <rdfs:label xml:lang="en">Copyright license</rdfs:label>
        <rdfs:comment xml:lang="en">Any individual license, with which a particular legal entity, the licensor, grants rights to another legal entity, the licensee.</rdfs:comment>
    </owl:Class>
    


    <!-- http://www.markosproject.eu/ontologies/licenses#CopyrightLicenseTemplate -->

    <owl:Class rdf:about="http://www.markosproject.eu/ontologies/licenses#CopyrightLicenseTemplate">
        <rdfs:label xml:lang="en">Copyright license template</rdfs:label>
        <rdfs:comment xml:lang="en">Any software license templates, such as GPL or BSD. A particular copyright  license can be an instance of such a template.</rdfs:comment>
    </owl:Class>
    


    <!-- http://www.markosproject.eu/ontologies/licenses#LicenseAssessment -->

    <owl:Class rdf:about="http://www.markosproject.eu/ontologies/licenses#LicenseAssessment">
        <rdfs:label xml:lang="en">License assessment</rdfs:label>
        <rdfs:comment xml:lang="en">Assessment of the compliance of a licence (see Object Property :assessment).</rdfs:comment>
    </owl:Class>
    


    <!-- http://www.markosproject.eu/ontologies/licenses#Work -->

    <owl:Class rdf:about="http://www.markosproject.eu/ontologies/licenses#Work">
        <rdfs:label xml:lang="en">Work</rdfs:label>
        <rdfs:comment xml:lang="en">&quot;Work&quot; means the literary and/or artistic work offered under the terms of this License including without limitation any production in the literary, scientific and artistic domain, whatever may be the mode or form of its expression including digital form, such as a book, pamphlet and other writing; a lecture, address, sermon or other work of the same nature; a dramatic or dramatico-musical work; a choreographic work or entertainment in dumb show; a musical composition with or without words; a cinematographic work to which are assimilated works expressed by a process analogous to cinematography; a work of drawing, painting, architecture, sculpture, engraving or lithography; a photographic work to which are assimilated works expressed by a process analogous to photography; a work of applied art; an illustration, map, plan, sketch or three-dimensional work relative to geography, topography, architecture or science; a performance; a broadcast; a phonogram; a compilation of data to the extent it is protected as a copyrightable work; or a work performed by a variety or circus performer to the extent it is not otherwise considered a literary or artistic work.</rdfs:comment>
    </owl:Class>
</rdf:RDF>



<!-- Generated by the OWL API (version 3.4.2) http://owlapi.sourceforge.net -->

